rocq-skylabs-brick/theories/lang/cpp/syntax/typing.v
@@ -290,6 +290,9 @@ Module decltype.
         | Estring chars t =>
             mret $ Tref $ Tarray (Tconst t) (1 + literal_string.lengthN chars)
         | Eint _ t => mret t
+        | Efloat ft _ t =>
+            let* _ := guard (t = Tfloat_ ft) in
+            mret t
         | Ebool _ => mret Tbool
         | Eunop _ _ t => mret t
         | Ebinop op l _ t => of_binop op l t
