rocq-skylabs-cpp2v/tests/cpp2v/test_float_lit.t/run.t
@@ -3,3 +3,7 @@
   cpp2v -v -check-types -names test_17_cpp_names.v -o test_17_cpp.v test.cpp -- -std=c++17 2>&1 | sed 's/^ *[0-9]* | //'
   coqc -w -notation-overridden -w -notation-incompatible-prefix test_17_cpp_names.v
   coqc -w -notation-overridden -w -notation-incompatible-prefix test_17_cpp.v
+  $ grep -o 'Efloat Ffloat (fp_of_bits Ffloat 1065353216%Z) Tfloat' test_17_cpp.v
+  Efloat Ffloat (fp_of_bits Ffloat 1065353216%Z) Tfloat
+  $ grep -o 'Efloat Fdouble (fp_of_bits Fdouble 4607182418800017408%Z) Tdouble' test_17_cpp.v
+  Efloat Fdouble (fp_of_bits Fdouble 4607182418800017408%Z) Tdouble
